ABI/Decode.lean
@@ -120,7 +120,16 @@ mutual
         let endOffset := payloadStart + paddedSize size
         zeroPadding? bytes (payloadStart + size) (paddedSize size - size)
         some (.bytes (ByteArray.mk payload.toArray), endOffset)
-    | .string => none
+    | .string => do
+        let size <- readNat? bytes start
+        if solcMaxU64 < size then
+          none
+        else
+        let payloadStart := start + 32
+        let payload <- readBytes? bytes payloadStart size
+        let endOffset := payloadStart + paddedSize size
+        zeroPadding? bytes (payloadStart + size) (paddedSize size - size)
+        some (.bytes (ByteArray.mk payload.toArray), endOffset)
     | .dynamicArray elemTy => do
         let size <- readNat? bytes start
         if solcMaxU64 < size then
